src/tls/experiments/ConnectionTable/ConnectionTable_Aux.fst
@@ -8,94 +8,60 @@ module S = Spec.Agile.AEAD
 module HS = FStar.HyperStack
 module HST = FStar.HyperStack.ST
 
-let connection_id = UInt8.t
-
-let configuration = UInt32.t
-
-let alg = S.AES128_GCM
-
-let cookie = c:AE.cipher_p alg
-  {B.length c == 64 + AE.iv_length + S.tag_length alg}
-
-let cookie_rgn = Mem.tls_define_region
-let table_rgn  = Mem.tls_tables_region
-let other_rgn  = Mem.tls_psk_region
-
-let random = Seq.lseq UInt8.t 32
-
-let id_of_random (r:random) : connection_id =
-  Seq.index r 0
-
-noeq
-type client_hello =
-  | CH1: random -> client_hello
-  | CH2: random -> ck:cookie{B.frameOf ck == other_rgn} -> client_hello
-
-let ch_random = function
-  | CH1 r -> r
-  | CH2 r _ -> r
-  
-let has_cookie = CH2?
-
-let get_cookie (ch:client_hello{has_cookie ch}) =
-  let CH2 _ cookie = ch in
-  cookie
-
-let ch_of_cookie (ch:client_hello{has_cookie ch}) =
-  let CH2 random _ = ch in
-  CH1 random
-
-val ch_compatible: ch:client_hello -> cfg:configuration -> bool
 let ch_compatible ch cfg = false
 
-let rgn = table_rgn
-
-let model = Flags.model && Flags.ideal_AEAD
-
-let maybe_id = if model then connection_id else unit
-
-noeq
-type connection =
-  | Init: cfg:configuration -> connection
-  | Sent_HRR: ch:client_hello -> connection
-  | Sent_ServerHello: ch:client_hello -> id1:maybe_id -> connection
-  | Complete: ch:client_hello -> id1:maybe_id -> connection
-
-let step (s1 s2:connection) : Type0 =
-  match s1, s2 with
-  | Init _, Sent_HRR _ -> True
-  | Init _, Sent_ServerHello _ _ -> True
-  | Sent_ServerHello ch id1, Complete ch' id1' -> ch == ch' /\ id1 == id1'
-  | _, _ -> False
-
-let rel : Preorder.preorder connection = FStar.ReflexiveTransitiveClosure.closure step
-
-// Store the ID rather than making it a parameter?
-let connection_ref (id:maybe_id) = 
-  r:HST.mmmref connection rel{HS.frameOf r `HS.extends` rgn}
-
-// References to connections live in pairwise disjoint regions
 let minv (m:T.partial_dependent_map maybe_id connection_ref) =
   forall id1 id2.{:pattern (Some? (DM.sel m id1)); (Some? (DM.sel m id2))}
     (id1 <> id2 /\ Some? (DM.sel m id1) /\ Some? (DM.sel m id2)) ==>
     HS.frameOf (Some?.v (DM.sel m id1)) `HS.disjoint` HS.frameOf (Some?.v (DM.sel m id2))
 
-unfold
-let _connection_table = T.t rgn maybe_id connection_ref minv
+let empty = T.empty
 
-unfold
-let connection_table = if model then _connection_table else unit
+val connection_inv:
+    T.imap maybe_id connection_ref minv
+  -> connection
+  -> Type0
+let connection_inv m c =
+  if model then
+    match c with
+    | Sent_ServerHello ch id1 | Complete ch id1 ->
+      if has_cookie ch then
+        match T.sel m id1 with
+        | Some c' ->
+          HST.token_p c' (fun h0 ->
+            Sent_HRR? (HS.sel h0 c') /\
+            ch_of_cookie ch == Sent_HRR?.ch (HS.sel h0 c'))
+        | _ -> False
+      else True
+    | _ -> True
+  else True
 
-let cookie_phi (table: connection_table) s = 
-  Seq.length s >= 32 /\
-  (if model then
-    let random = Seq.slice s 0 32 in
-    let id = id_of_random random in
-    let t:_connection_table = table in
-    HST.token_p t (fun h -> 
-      T.defined t id h /\
-      (let c = T.value_of t id h in
-      HST.token_p c (fun h' -> 
-        Sent_HRR? (HS.sel h' c) /\
-        CH1 random == Sent_HRR?.ch (HS.sel h' c))))
-   else True)
+(*
+  Stateful invariant
+  Can't be attached to the table because it needs to dereference connections
+*)
+let inv t h =
+  h `HS.contains` t /\
+  (let m = HS.sel h t in
+  forall (id:maybe_id).{:pattern (T.defined t id h)}
+    (T.defined t id h /\ h `HS.contains` (T.value_of t id h))
+    ==> connection_inv m (HS.sel h (Some?.v (T.sel m id))))
+
+let framing h0 t l h1 =
+  assert (B.loc_includes (B.loc_all_regions_from true rgn) (B.loc_mreference t));
+  assert (forall (id:maybe_id).{:pattern (T.defined t id h1)}
+    (T.defined t id h1 /\ h1 `HS.contains` (T.value_of t id h1)) ==>
+    B.loc_includes (B.loc_all_regions_from true rgn) 
+                   (B.loc_mreference (T.value_of t id h1)));
+  assert (forall (id:maybe_id).{:pattern (T.defined t id h1)}
+    (T.defined t id h0 /\ h0 `HS.contains` (T.value_of t id h1)) ==>
+    B.loc_includes (B.loc_all_regions_from true rgn) 
+                   (B.loc_mreference (T.value_of t id h0)))
+
+let alloc _ =
+  if model then T.alloc () <: _connection_table
+
+let table = 
+  HST.recall_region rgn;
+  HST.witness_region rgn;
+  alloc ()
